src/go_lang/notation.v
@@ -87,6 +87,7 @@ Notation "()" := LitUnit : val_scope.
 Notation "! e" := (Load e%E) (at level 9, right associativity) : expr_scope.
 Notation "'ref' e" := (Alloc e%E) (at level 10) : expr_scope.
 Notation "- e" := (UnOp MinusUnOp e%E) : expr_scope.
+Notation "'to_u64' e" := (UnOp ToUInt64Op e%E) (at level 10) : expr_scope.
 
 Notation "e1 + e2" := (BinOp PlusOp e1%E e2%E) : expr_scope.
 Notation "e1 +ₗ e2" := (BinOp OffsetOp e1%E e2%E) : expr_scope.
